Utilities/Misc.thy
@@ -5,10 +5,17 @@ begin
 primrec map_fst :: "('a \<Rightarrow> 'c) \<Rightarrow> 'a \<times> 'b \<Rightarrow> 'c \<times> 'b" where
   "map_fst f (a, b) = (f a, b)"
 
+primrec index_of :: "'a \<Rightarrow> 'a list \<Rightarrow> nat" where
+  "index_of a [] = undefined"
+| "index_of a (a' # as) = (if a = a' then 0 else Suc (index_of a as))"
+
 lemma [simp]: "(x::nat) \<ge> y \<Longrightarrow> \<exists>z. x = y + z"
   proof (induction x arbitrary: y)
   case Suc
     thus ?case by (induction y) simp_all
   qed simp_all
+
+lemma [simp]: "(\<forall>x y. f x = f y \<longrightarrow> x = y) \<Longrightarrow> index_of (f a) (map f as) = index_of a as"
+  by (induction as) simp_all
 
 end
